src/PlutusIR/Semantics/SemanticEquivalence/LogicalRelation/RC/Helpers.v
@@ -20,3 +20,30 @@ Proof.
   eapply H0.
   assumption.
 Qed.
+
+
+(* Run an C(e, e') by looking in the context for an evaluation of e, and use that
+* amount of steps
+* binds the resulting
+*    r' : result
+*    j' : nat
+*    H_eval' : eval e' ... 
+*    H_res' : V(r, r')
+*)
+Ltac run_C H_RC r' j' H_eval' H_res':=
+  match type of H_RC with
+  | C ?k ?T ?ρ ?e1 ?e2 =>
+    match goal with
+    | H_ev : e1 =[ ?i ]=> ?v1 |- _ =>
+        let H_RC' := fresh "H" in
+        let H_ev'  := fresh "H_ev" in
+        assert (H_RC' := H_RC); assert (H_ev' := H_ev);
+
+        autorewrite with R in H_RC';
+        apply H_RC' in H_ev' as [r' [j' [H_eval' H_res']]];
+        clear H_RC'
+    | _ =>
+      fail 1 "Could not find required hypothesis of type eval"
+    end
+  end
+.
