src/PlutusIR/Semantics/SemanticEquivalence/LogicalRelation/RD/Helpers.v
@@ -34,6 +34,34 @@ Proof.
       eapply IHRD; eauto.
 Qed.
 
+
+Lemma D_Rel : forall ck rho,
+    D ck rho ->
+    forall X Chi T1 T2,
+      sem rho X = Datatypes.Some Chi ->
+      syn1 rho X = Datatypes.Some T1 ->
+      syn2 rho X = Datatypes.Some T2 ->
+      Rel' T1 T2 Chi.
+Proof.
+  induction 1.
+  - intros.
+    unfold sem in H.
+    inversion H.
+  - intros.
+    unfold sem in H3.
+    unfold syn1 in H4.
+    unfold syn2 in H5.
+    destruct (X0 =? X) eqn:Heqb.
+    + inversion H3. subst.
+      inversion H4. subst.
+      inversion H5. subst.
+      assumption.
+    + fold sem in H3.
+      fold syn1 in H4.
+      fold syn2 in H5.
+      eapply IHD; eauto.
+Qed.
+
 Lemma RD_sem_syn : forall ck rho,
     RD ck rho ->
     forall X Chi,
@@ -52,6 +80,23 @@ Proof.
     destruct (X0 =? X) eqn:Heqb; eauto.
 Qed.
 
+Lemma D_sem_syn : forall ck rho,
+    D ck rho ->
+    forall X Chi,
+      sem rho X = Datatypes.Some Chi ->
+      exists T1 T2,
+        syn1 rho X = Datatypes.Some T1 /\
+        syn2 rho X = Datatypes.Some T2.
+Proof.
+  induction 1.
+  - intros.
+    unfold sem in H.
+    inversion H.
+  - intros.
+    unfold sem in H3.
+    simpl.
+    destruct (X0 =? X) eqn:Heqb; eauto.
+Qed.
 
 Lemma RD_sem_Rel ck rho :
     RD ck rho ->
@@ -67,8 +112,43 @@ Proof with eauto.
   eapply RD_Rel...
 Qed.
 
+
+Lemma D_sem_Rel ck rho :
+    D ck rho ->
+    forall X χ,
+      sem rho X = Some χ ->
+      exists T1 T2,
+      Rel' T1 T2 χ.
+Proof with eauto.
+  intros H_D X Chi H_sem.
+  assert (H_sem' := H_sem).
+  apply D_sem_syn with (ck := ck) in H_sem' as [ T1 [ T2 [H_syn1 H_syn2] ]]...
+  exists T1, T2.
+  eapply D_Rel...
+Qed.
+
 Lemma RD_syn_closed : forall ck rho,
     RD ck rho ->
+      forall X T1 T2,
+        syn1 rho X = Datatypes.Some T1 ->
+        syn2 rho X = Datatypes.Some T2 ->
+        Ty.closed T1 /\ Ty.closed T2.
+Proof with eauto.
+  induction 1; intros...
+  - discriminate.
+  - simpl in H3.
+    simpl in H4.
+    destruct (X0 =? X).
+    + inversion H3; subst.
+      inversion H4; subst.
+      split.
+      all: eauto using Ty.kindable_empty__closed.
+    + eauto.
+Qed.
+
+
+Lemma D_syn_closed : forall ck rho,
+    D ck rho ->
       forall X T1 T2,
         syn1 rho X = Datatypes.Some T1 ->
         syn2 rho X = Datatypes.Some T2 ->
